doc/coq/Sound.v
@@ -1,5 +1,38 @@
-From MODULAR Require Import Abstract.
-From MODULAR Require Import Concrete.
+From MODULAR Require Export Abstract.
+From MODULAR Require Export Concrete.
+Require Export Coq.Logic.FunctionalExtensionality.
+
+Fixpoint list_to_mem l :=
+  match l with
+  | [] => Concrete.empty_mem
+  | (addr, (Val v pf Cv)) :: tl => 
+    (addr !-> (Val v pf Cv) ; (list_to_mem tl))
+  end.
+
+Fixpoint increasing (l : list (prod path expr_value)) :=
+  match l with
+  | [] => True
+  | [(t :: _, _)] => True
+  | (t1 :: _, _) :: 
+    (t2 :: _, _) :: tl => (t1 > t2) /\ increasing tl
+  | _ => False
+  end.
+
+Definition finite_mem mem :=
+  exists l, mem = list_to_mem l /\ increasing l.
+
+Fixpoint sound_addr C mem_list abs_C abs_mem : Prop :=
+  Concrete.dy_to_st C = Abstract.dy_to_st abs_C /\
+  forall x,
+    match mem_list with
+    | [] => True
+    | (addr, Val v pf Cv) :: tl =>
+      if eq_p addr (addr_x C x) 
+      then exists abs_Cv, 
+        (In (Abstract.Val v pf abs_Cv) (abs_mem (Abstract.addr_x abs_C x))) /\
+        sound_addr Cv tl abs_Cv abs_mem
+      else sound_addr C tl abs_C abs_mem
+    end.
 
 Theorem soundness :
   forall e C' st' e'
